More fail instances

Classes/Monad/MonadExcept.v
@@ -6,13 +6,13 @@ Require Import Classes.Monad.MonadFail.
 Implicit Type M : Type → Type.
 Implicit Type A : Type.
 
-Class MonadExcept M `{MonadFail M} := {
-  catch : forall {A}, M A -> M A -> M A;
-  catch_left : forall {A} (x : M A), catch fail x = x;
-  catch_right : forall {A} (x : M A), catch x fail = x;
-  catch_assoc : ∀ {A} (x y z: M A),
+Class MonadExcept M `{MonadFail M} A := {
+  catch : M A -> M A -> M A;
+  catch_left : ∀ (x : M A), catch fail x = x;
+  catch_right : ∀ (x : M A), catch x fail = x;
+  catch_assoc : ∀ (x y z: M A),
     catch x (catch y z) = catch (catch x y) z;
-  catch_pure : ∀ {A} (x : M A) (a : A),
+  catch_pure : ∀ (x : M A) (a : A),
     catch (pure a) x = pure a;
 }.
 Arguments catch : simpl never.
