Instances/Except.v
@@ -33,35 +33,97 @@ Section except_maybe.
     end.
   Hint Unfold catch_maybe : soundness.
 
-  Lemma catch_maybe_throw_left : ∀ A (x : Maybe A),
+  Lemma catch_maybe_throw_left : ∀ {A} (x : Maybe A),
     catch_maybe None x = x.
   Proof. simple_solve. Qed.
 
-  Lemma catch_maybe_throw_right : ∀ A (x : Maybe A),
+  Lemma catch_maybe_throw_right : ∀ {A} (x : Maybe A),
     catch_maybe x None = x.
   Proof. simple_solve. Qed.
 
-  Lemma catch_maybe_assoc  : ∀ (A : Type) (x y z : Maybe A),
+  Lemma catch_maybe_assoc  : ∀ {A : Type} (x y z : Maybe A),
     catch_maybe x (catch_maybe y z) = catch_maybe (catch_maybe x y) z.
   Proof.
     intros. destruct_all (Maybe A); reflexivity.
   Qed.
 
-  Lemma catch_maybe_pure : ∀ (A : Type) (x : Maybe A) (a : A),
+  Lemma catch_maybe_pure : ∀ {A : Type} (x : Maybe A) (a : A),
     catch_maybe (pure a) x = pure a.
   Proof.
     reflexivity. 
   Qed.
 
-  Global Instance except_maybe : MonadExcept Maybe :=
+  Global Instance except_maybe : ∀ A, MonadExcept Maybe A :=
   {
-    catch := @catch_maybe;
+    catch := catch_maybe;
     catch_left := catch_maybe_throw_left;
     catch_right := catch_maybe_throw_right;
     catch_assoc := catch_maybe_assoc;
     catch_pure := catch_maybe_pure;
   }.
 End except_maybe.
+
+Section fail_abstract_maybe.
+  Lemma noneA_left : ∀ (A B : Type) (f : A → AbstractMaybe B), 
+     (@NoneA A) >>= f = NoneA.
+  Proof.
+    simple_solve.
+  Qed.
+
+  Global Instance fail_abstract_maybe : MonadFail AbstractMaybe :=
+  {
+    fail := @NoneA;
+    fail_left := noneA_left;
+  }.
+End fail_abstract_maybe.
+
+Section except_abstract_maybe.
+  Context {A} `{Joinable A}.
+  Definition catch_abstract_maybe (x y : AbstractMaybe A) : AbstractMaybe A :=
+    match x with
+    | NoneA => y
+    | JustA a => x 
+    | JustOrNoneA a => join_op x y
+    end.
+
+  Lemma catch_abstract_maybe_throw_left : ∀ (x : AbstractMaybe A),
+    catch_abstract_maybe NoneA x = x.
+  Proof. reflexivity. Qed.
+
+  Lemma catch_abstract_maybe_throw_right : ∀ (x : AbstractMaybe A),
+    catch_abstract_maybe x NoneA = x.
+  Proof.
+    intros. destruct x; simpl. 2: unfold join_op; simpl. 
+  Admitted.
+
+  Lemma catch_abstract_maybe_pure : ∀ (x : AbstractMaybe A) (a : A),
+    catch_abstract_maybe (pure a) x = pure a.
+  Proof.
+    reflexivity. 
+  Qed.
+
+  Lemma catch_abstract_maybe_assoc : ∀ (x y z : AbstractMaybe A),
+    catch_abstract_maybe x (catch_abstract_maybe y z) =
+    catch_abstract_maybe (catch_abstract_maybe x y) z.
+  Proof.
+    intros. destruct x as [a1|a1|] eqn:Hx; 
+    destruct y as [a2|a2|] eqn:Hy; 
+    destruct z as [a3|a3|] eqn:Hz; simpl; try reflexivity.
+    - unfold join_op; simpl. admit.
+    - unfold join_op; simpl. admit.
+    - unfold join_op; simpl. admit.
+    - unfold join_op; simpl. rewrite join_assoc. reflexivity.
+  Admitted.
+
+  Global Instance fail_maybeA : MonadExcept AbstractMaybe A :=
+  {
+    catch := catch_abstract_maybe;
+    catch_left := catch_abstract_maybe_throw_left;
+    catch_right := catch_abstract_maybe_throw_right;
+    catch_pure := catch_abstract_maybe_pure;
+    catch_assoc := catch_abstract_maybe_assoc;
+  }.
+End except_abstract_maybe.
 
 Section fail_maybeT.
   Context {M} `{inst : Monad M}.
@@ -93,14 +155,14 @@ Section except_maybeT.
       end).
   Hint Unfold catch_maybeT : soundness.
 
-  Lemma catch_maybeT_throw_left : ∀ (A : Type) (x : MaybeT M A), 
+  Lemma catch_maybeT_throw_left : ∀ {A : Type} (x : MaybeT M A), 
     catch_maybeT fail_maybeT x = x.
   Proof.
     intros. unfold catch_maybeT, fail_maybeT.
     autorewrite with soundness. reflexivity.
   Qed.
 
-  Lemma catch_maybeT_throw_right : ∀ (A : Type) (x : MaybeT M A), 
+  Lemma catch_maybeT_throw_right : ∀ {A : Type} (x : MaybeT M A), 
     catch_maybeT x fail_maybeT = x.
   Proof.
     unfold catch_maybeT, fail_maybeT. intros.
@@ -109,7 +171,7 @@ Section except_maybeT.
     rewrite <- (bind_id_right (M:=M)). f_equal.
   Qed.
 
-  Lemma catch_maybeT_assoc : ∀ (A : Type) (x y z : MaybeT M A),
+  Lemma catch_maybeT_assoc : ∀ {A : Type} (x y z : MaybeT M A),
     catch_maybeT x (catch_maybeT y z) = catch_maybeT (catch_maybeT x y) z.
   Proof.
     intros. unfold catch_maybeT. autorewrite with soundness. f_equal. 
@@ -117,18 +179,18 @@ Section except_maybeT.
     f_equal.
   Qed.
 
-  Lemma catch_maybeT_pure : ∀ (A : Type) (x : MaybeT M A) (a : A),
+  Lemma catch_maybeT_pure : ∀ {A : Type} (x : MaybeT M A) (a : A),
     catch_maybeT (pure a) x = pure a.
   Proof.
     unfold catch_maybeT. intros. unfold pure; simpl; unfold pure_maybeT. 
     rewrite bind_id_left. reflexivity.
   Qed.
 
-  Global Instance except_maybeT : MonadExcept (MaybeT M) :=
+  Global Instance except_maybeT {A} : MonadExcept (MaybeT M) A :=
   {
-    catch := @catch_maybeT;
-    catch_left := @catch_maybeT_throw_left;
-    catch_right := @catch_maybeT_throw_right;
+    catch := catch_maybeT;
+    catch_left := catch_maybeT_throw_left;
+    catch_right := catch_maybeT_throw_right;
     catch_assoc := catch_maybeT_assoc;
     catch_pure := catch_maybeT_pure;
   }. 
@@ -165,21 +227,21 @@ Section except_maybeAT.
       | NoneA => my
       end).
 
-  Lemma catch_maybeAT_throw_left : ∀ A (x : MaybeAT M A),
+  Lemma catch_maybeAT_throw_left : ∀ {A} (x : MaybeAT M A),
     catch_maybeAT fail_maybeAT x = x.
   Proof. 
     intros. unfold catch_maybeAT, fail_maybeAT. autorewrite with soundness.
     reflexivity.
   Qed.
 
-  Lemma catch_maybeAT_throw_right : ∀ A (x : MaybeAT M A),
+  Lemma catch_maybeAT_throw_right : ∀ {A} (x : MaybeAT M A),
     catch_maybeAT x fail_maybeAT = x.
   Proof. 
     intros. unfold catch_maybeAT, fail_maybeAT. rewrite <- (bind_id_right (M:=M)).
     f_equal; extensionality m. destruct m; reflexivity.
   Qed.
 
-  Lemma catch_maybeAT_assoc : ∀ (A : Type) (x y z : MaybeAT M A),
+  Lemma catch_maybeAT_assoc : ∀ {A} (x y z : MaybeAT M A),
     catch_maybeAT x (catch_maybeAT y z) = catch_maybeAT (catch_maybeAT x y) z.
   Proof.
     intros. unfold catch_maybeAT. rewrite bind_assoc. f_equal. 
@@ -187,16 +249,16 @@ Section except_maybeAT.
     f_equal.
   Qed.
 
-  Lemma catch_maybeAT_pure : ∀ (A : Type) (x : MaybeAT M A) (a : A),
+  Lemma catch_maybeAT_pure : ∀ {A} (x : MaybeAT M A) (a : A),
     catch_maybeAT (pure a) x = pure a.
   Proof.
     unfold catch_maybeAT. intros. unfold pure; simpl; unfold pure_maybeAT. 
     rewrite bind_id_left. reflexivity.
   Qed.
 
-  Global Instance except_maybeAT : MonadExcept (MaybeAT M) :=
+  Global Instance except_maybeAT {A} : MonadExcept (MaybeAT M) A :=
     {
-      catch := @catch_maybeAT;
+      catch := catch_maybeAT;
       catch_left := catch_maybeAT_throw_left;
       catch_right := catch_maybeAT_throw_right;
       catch_assoc := catch_maybeAT_assoc;
@@ -227,43 +289,43 @@ Section fail_stateT.
 End fail_stateT.
 
 Section except_stateT.
-  Context {M : Type → Type} `{MonadExcept M}.
+  Context {M : Type → Type} `{MonadFail M} `{∀ A, MonadExcept M A}.
   Context {S : Type}.
 
   Definition catch_stateT {A} (a b : StateT S M A) : StateT S M A := 
     fun s => catch (a s) (b s).
   Hint Unfold fail_stateT catch_stateT : soundness.
 
-  Lemma catch_stateT_throw_left : ∀ A (x : StateT S M A),
+  Lemma catch_stateT_throw_left : ∀ {A} (x : StateT S M A),
     catch_stateT fail_stateT x = x.
   Proof. 
     intros. unfold catch_stateT, fail_stateT, lift_stateT.
     ext. autorewrite with soundness. reflexivity.
   Qed.
 
-  Lemma catch_stateT_throw_right : ∀ A (x : StateT S M A),
+  Lemma catch_stateT_throw_right : ∀ {A} (x : StateT S M A),
     catch_stateT x fail_stateT = x.
   Proof. 
     intros. unfold catch_stateT, fail_stateT, lift_stateT.
     ext. autorewrite with soundness. reflexivity.
   Qed.
 
-  Lemma catch_stateT_assoc : ∀ A (x y z: StateT S M A),
+  Lemma catch_stateT_assoc : ∀ {A} (x y z: StateT S M A),
     catch_stateT x (catch_stateT y z) = catch_stateT (catch_stateT x y) z.
   Proof.
     intros. unfold catch_stateT. ext. rewrite catch_assoc. reflexivity.
   Qed.
 
-  Lemma catch_stateT_pure : ∀ A (x : StateT S M A) (a : A),
+  Lemma catch_stateT_pure : ∀ {A} (x : StateT S M A) (a : A),
     catch_stateT (pure a) x = pure a.
   Proof.
     intros. unfold catch_stateT. ext. unfold pure. simpl. unfold pure_stateT.
     rewrite catch_pure. reflexivity.
   Qed.
 
-  Instance except_stateT : MonadExcept (StateT S M) :=
+  Instance except_stateT {A} : MonadExcept (StateT S M) A :=
   {
-    catch := @catch_stateT;
+    catch := catch_stateT;
     catch_left := catch_stateT_throw_left;
     catch_right := catch_stateT_throw_right;
     catch_assoc := catch_stateT_assoc;
