Classes/SoundMonad.v
@@ -4,16 +4,17 @@ Require Import Classes.Galois.
 Require Import Classes.Functor.
 Require Import Classes.Applicative.
 Require Import Classes.Monad.
+Require Import Classes.Monad.MonadFail.
 Require Import Instances.Galois.
 
 Section sound_monad.
-  Context (M M' : Type → Type) `{Monad M, Monad M'}.
+  Context (M M' : Type → Type) `{MonadFail M, MonadFail M'}.
   Context {M_preorder : ∀ T', PreorderedSet T' → PreorderedSet (M' T')}.
   Context {M_galois : ∀ T T' {HT : PreorderedSet T'}, Galois T T' → Galois (M T) (M' T')}.
 
   Class SoundMonad : Type :=
   {
-    fmap_sound : ∀ (A A' B B' : Type ) `{Galois A A', Galois B B'},
+    fmap_sound : ∀ (A A' B B' : Type) `{Galois A A', Galois B B'},
       gamma (fmap (F:=M') (A:=A') (B:=B')) (fmap (F:=M) (A:=A) (B:=B));
     pure_sound : ∀ (A A' : Type) `{Galois A A'},
       gamma (pure (F:=M') (A:=A')) (pure (F:=M) (A:=A));
@@ -21,6 +22,7 @@ Section sound_monad.
       gamma (app (F:=M') (A:=A') (B:=B')) (app (F:=M) (A:=A) (B:=B));
     bind_sound : ∀ (A A' B B' : Type) `{Galois A A', Galois B B'},
       gamma (bindM (M:=M') (A:=A') (B:=B')) (bindM (M:=M) (A:=A) (B:=B));
+    gamma_fail : ∀ (A A' : Type) `{Galois A A'} (m : M A), gamma fail m;
   }.
 End sound_monad.
-Hint Resolve fmap_sound pure_sound app_sound bind_sound : soundness.
+Hint Resolve fmap_sound pure_sound app_sound bind_sound gamma_fail : soundness.
